tune

Weidenbach_Book/Array_UInt.thy
@@ -148,7 +148,41 @@ lemma arrayO_arl_get_u_rule[sep_heap_rules]:
       uint32_nat_rel_def br_def)
 
 
-code_printing constant arl_get_u \<rightharpoonup> (SML) "(fn/ ()/ =>/ Array.sub/ (fst (_),/ Word32.toInt (_)))"
+definition arl_swap_u_code
+  :: "'a ::heap array_list \<Rightarrow> uint32 \<Rightarrow> uint32 \<Rightarrow> 'a array_list Heap"
+where
+  \<open>arl_swap_u_code xs i j = do {
+     ki \<leftarrow> arl_get_u xs i;
+     kj \<leftarrow> arl_get_u xs j;
+     xs \<leftarrow> arl_set_u xs i kj;
+     xs \<leftarrow> arl_set_u xs j ki;
+     return xs
+  }\<close>
+
+lemma arl_op_list_swap_u_hnr[sepref_fr_rules]:
+  assumes p: \<open>CONSTRAINT is_pure R\<close>
+  shows \<open>(uncurry2 arl_swap_u_code, uncurry2 (RETURN ooo op_list_swap)) \<in>
+       [\<lambda>((xs, i), j).  i < length xs \<and> j < length xs]\<^sub>a
+      (arl_assn R)\<^sup>d *\<^sub>a uint32_nat_assn\<^sup>k  *\<^sub>a uint32_nat_assn\<^sup>k \<rightarrow> arl_assn R\<close>
+proof -
+  obtain R' where R: \<open>the_pure R = R'\<close> and R': \<open>R = pure R'\<close>
+    using p by fastforce
+    find_theorems \<open>arl_assn\<close> arl_get
+  show ?thesis
+  by (sepref_to_hoare)
+    (sep_auto simp: arl_swap_u_code_def swap_def nth_u_code_def is_array_def
+      array_assn_def hr_comp_def nth_nat_of_uint32_nth'[symmetric]
+      list_rel_imp_same_length uint32_nat_rel_def br_def arl_assn_def
+      heap_array_set_u_def heap_array_set'_u_def Array.upd'_def 
+      arl_set'_u_def R R'
+      nat_of_uint32_code[symmetric] R arl_set_u_def arl_get'_def arl_get_u_def
+      intro!: list_rel_update[of _ _ R true _ _ \<open>(_, {})\<close>, unfolded R] param_nth)
+qed
+
+definition arl_get_u' where
+  [symmetric, code]: \<open>arl_get_u' = arl_get_u\<close>
+
+code_printing constant arl_get_u' \<rightharpoonup> (SML) "(fn/ ()/ =>/ Array.sub/ (fst (_),/ Word32.toInt (_)))"
 
 lemma arl_get'_nth'[code]: \<open>arl_get' = (\<lambda>(a, n). Array.nth' a)\<close>
   unfolding arl_get_def arl_get'_def Array.nth'_def
